fix erros in definitions

src/mcl.lean
@@ -43,7 +43,17 @@ def create_signature : list (string × variable_def) → signature
 def type_map : type → Type
 | int := ℕ
 | float := ℕ
-| bool := bool
+| bool := _root_.bool
+
+instance (t) : inhabited (type_map t) := ⟨
+    match t with 
+    | type.int := 0
+    | type.float := 0
+    | type.bool := ff
+    end
+⟩
+
+#eval default (type_map int)
 
 @[reducible]
 def type_of : variable_def → type := λ v, v.type.type
@@ -99,6 +109,8 @@ instance (t : type) : has_add (expression sig t) := ⟨expression.add⟩
 instance : has_zero (expression sig int) := ⟨expression.const_int 0 rfl⟩
 instance : has_one (expression sig int) := ⟨expression.const_int 1 rfl⟩
 infix < := expression.lt (show type.bool = type.bool, by refl)
+notation `v(` n `)`:= expression.tlocal_var n (by refl)
+notation `i(` n `)`:= expression.const_int n (by refl)
 
 def type_map_add : Π{t : type}, type_map t → type_map t → type_map t
 | int a b := a + b
@@ -109,7 +121,7 @@ def type_map_add : Π{t : type}, type_map t → type_map t → type_map t
 #reduce type.sizeof int
 #check type.no_confusion_type
 
-#reduce expression.sizeof (λ_, { scope := scope.tlocal, type := type.int}) int (add (const_int 4 (by refl)) (const_int 5 (by refl)))
+#reduce expression.sizeof (λ_, { scope := scope.tlocal, type := ⟨_, [1], type.int⟩}) int (add (const_int 4 (by refl)) (const_int 5 (by refl)))
 #print expression.sizeof
 
 #check @well_founded.fix
@@ -120,8 +132,9 @@ def subterm (q : Σ t : type, expression sig t) : (Σ t : type, expression sig t
 | ⟨t, lt _ a b⟩ := subterm ⟨int, a⟩ ∨ subterm ⟨int, b⟩
 | t := t = q
 
-example : well_founded (subterm) := begin
+example {sig : signature} : well_founded (@subterm sig) := begin
     apply well_founded.intro,
+    sorry,
 end
 
 #print expression.sizeof
@@ -129,13 +142,13 @@ end
 @[reducible, simp] 
 def expression_size {sig : signature} : Π {t : type}, expression sig t → ℕ
 | t (const_int _ _) := 1
-| t (tlocal_var _ _ _ _) := 1
-| t (global_var _ _ _) := 1
+| t (tlocal_var _ _ _ _ _) := 1
+| t (global_var _ _ _ _ _) := 1
 | t (add a b) := 
     have a.sizeof sig t < (add a b).sizeof sig t := begin
         rw expression.sizeof,
         simp,
-        
+        sorry,
     end,
     have b.sizeof sig t < (add a b).sizeof sig t := sorry,
     expression_size a + expression_size b
@@ -162,19 +175,6 @@ def eval {sig : signature} (s : state sig) : Π {t : type}, expression sig t →
 --     end)⟩], 
 -- /- dec_tac := do tactic.interactive.simp -/ }
 
-#print eval
-#print eval._main
-
-example (s : state sig) (t) (a b : expression sig int) (h) : eval._match_1 ⟨int, ⟨s, b⟩⟩ < mcl.eval._match_1 ⟨t, ⟨s, lt h a b⟩⟩
-:= begin
-    --unfold eval._match_1,
-    -- rw expression_size,
-    simp [eval._match_1],
-end
-
-#print eval
-#print eval._main
-#print eval._main._pack
 
 -- if we compare two variable accesses to the same array: when using vectors we only have to reason about equality of elements, otherwise we have to reason about length as well
 @[reducible]
@@ -190,25 +190,37 @@ def load_global_vars_for_expr {sig : signature} : Π {t : type}, expression sig 
 | t (lt _ a b) := load_global_vars_for_expr a ++ load_global_vars_for_expr b
 
 def prepend_load_expr {sig : signature} {t : type} (expr : expression sig t) (k : parlang_mcl_kernel sig) :=
-list_to_kernel_seq (load_global_vars_for_expr expr ++ [k])
+(load_global_vars_for_expr expr).foldr (λ k₁ k₂, k₁ ;; k₂) k
+--list_to_kernel_seq (load_global_vars_for_expr expr ++ [k])
 
 def append_load_expr  {sig : signature} {t : type} (expr : expression sig t) (k : parlang_mcl_kernel sig) :=
-list_to_kernel_seq ([k] ++ load_global_vars_for_expr expr)
+(load_global_vars_for_expr expr).foldl (λ k₁ k₂, k₁ ;; k₂) k
+--list_to_kernel_seq ([k] ++ load_global_vars_for_expr expr)
+
+example (k) : prepend_load_expr (7 : expression sig int) k = k := by refl
+example (k) (n idx h₁ h₂ h₃) : prepend_load_expr (@global_var sig _ 1 n idx h₁ h₂ h₃ : expression sig int) k = k := begin
+    rw prepend_load_expr,
+    rw load_global_vars_for_expr,
+    repeat { rw list.foldr },
+    sorry
+end
+
+example (k) : append_load_expr (7 : expression sig int) k = k := by refl
+example (k) (n idx h₁ h₂ h₃) : append_load_expr (@global_var sig _ 1 n idx h₁ h₂ h₃ : expression sig int) k = k := begin
+    rw append_load_expr,
+    rw load_global_vars_for_expr,
+    repeat { rw list.foldl },
+    sorry
+end
 
 -- TODO prove lemma
 -- eval expression (specifically the loads only influence the expression)
 -- prove more lemmas to make sure loads are placed correctly
 -- do I need a small step seantic for this?
 
-notation `v(` n `)`:= expression.tlocal_var n (by refl)
-infixr ` ~+ `:90 := expression.add
-notation `i(` n `)`:= expression.const_int n (by refl)
-
-open expression
-
 def expr_reads (n : string) : Π {t : type}, expression sig t → Prop
-| t (tlocal_var m _ _ _) := m = n
-| t (global_var m _ _) := m = n
+| t (tlocal_var m _ _ _ _) := m = n
+| t (global_var m _ _ _ _) := m = n
 | t (add expr₁ expr₂) := expr_reads expr₁ ∨ expr_reads expr₂
 | t (const_int _ _) := false
 | t (lt _ a b) := expr_reads a ∨ expr_reads b
@@ -217,7 +229,7 @@ inductive mclk (sig : signature)
 | tlocal_assign {dim : ℕ} (n : string) (idx : vector (expression sig int) dim) (h : (sig n).type.dim = idx.length) : (expression sig (type_of (sig n))) → mclk
 | global_assign {dim : ℕ} (n) (idx : vector (expression sig int) dim) (h : (sig n).type.dim = idx.length) : (expression sig (type_of (sig n))) → mclk
 | seq : mclk → mclk → mclk
-| for (n : string) (h : sig.type_of n = int) :
+| for (n : string) (h : sig.type_of n = int) (h₂ : (sig n).type.dim = 1) :
   expression sig int → expression sig bool → mclk → mclk → mclk
 | skip {} : mclk
 
@@ -226,20 +238,20 @@ infixr ` ;; `:90 := mclk.seq
 open mclk
 
 def mclk_reads (n : string) : mclk sig → Prop
-| (tlocal_assign _ expr) := expr_reads n expr
-| (global_assign _ expr) := expr_reads n expr
+| (tlocal_assign _ idx _ expr) := expr_reads n expr -- todo add idx in usages
+| (global_assign _ idx _ expr) := expr_reads n expr
 | (seq k₁ k₂) := mclk_reads k₁ ∨ mclk_reads k₂
-| (for _ _ init c inc body) := expr_reads n init ∨ expr_reads n c ∨ mclk_reads inc ∨ mclk_reads body
-| (skip _) := false
+| (for _ _ _ init c inc body) := expr_reads n init ∨ expr_reads n c ∨ mclk_reads inc ∨ mclk_reads body
+| (skip) := false
 
 --lemma mclk_expr_reads (k) : mclk_reads n k → ∃ expr, (expr_reads n expr ∧ subexpr expr k)
 
 def mclk_to_kernel {sig : signature} : mclk sig → parlang_mcl_kernel sig
 | (seq k₁ k₂) := kernel.seq (mclk_to_kernel k₁) (mclk_to_kernel k₂)
-| (skip _) := kernel.compute id
+| (skip) := kernel.compute id
 | (tlocal_assign n idx h expr) := prepend_load_expr expr (kernel.compute (λ s : state sig, s.update' (show type_of (sig n) = type_of (sig n), by refl) (show (sig n).type.dim = (idx.map (eval s)).length, from h) (eval s expr)))
 | (global_assign n idx h expr) := prepend_load_expr expr (kernel.compute (λ s, s.update' (show type_of (sig n) = type_of (sig n), by refl) (show (sig n).type.dim = (idx.map (eval s)).length, from h) (eval s expr))) ;; kernel.store (λ s, ⟨(n, (idx.map (eval s)).to_list), s.get' (show type_of (sig n) = type_of (sig n), by refl) (show (sig n).type.dim = (idx.map (eval s)).length, from h)⟩)
-| (for n h expr c k_inc k_body) := prepend_load_expr expr (kernel.compute (λ s, s.update' h (eval s expr))) ;; 
+| (for n h h₂ expr c k_inc k_body) := prepend_load_expr expr (kernel.compute (λ s, s.update' h (show (sig n).type.dim = (([0] : vector (expression sig int) _).map (eval s)).length, from h₂) (eval s expr))) ;; 
     prepend_load_expr c (
         kernel.loop (λ s, eval s c) (mclk_to_kernel k_body ;; append_load_expr c (mclk_to_kernel k_inc))
     )
@@ -304,15 +316,15 @@ end
 def state_assert (sig₁ sig₂ : signature) := Π n₁:ℕ, parlang.state n₁ (state sig₁) (λ n, type_map (sig₁.type_of n)) → vector bool n₁ → Π n₂:ℕ, parlang.state n₂ (state sig₂) (λ n, type_map (sig₂.type_of n)) → vector bool n₂ → Prop
 
 def mclk_rel {sig₁ sig₂ : signature} 
-    (P : Π n₁:ℕ, parlang.state n₁ (state sig₁) (λ n, (sig₁.lean_type_of n)) → vector bool n₁ → Π n₂:ℕ, parlang.state n₂ (state sig₂) (λ n, (sig₂.lean_type_of n)) → vector bool n₂ → Prop)
+    (P : Π n₁:ℕ, parlang.state n₁ (state sig₁) (parlang_mcl_global sig₁) → vector bool n₁ → Π n₂:ℕ, parlang.state n₂ (state sig₂) (parlang_mcl_global sig₂) → vector bool n₂ → Prop)
     (k₁ : mclk sig₁) (k₂ : mclk sig₂)
-    (Q : Π n₁:ℕ, parlang.state n₁ (state sig₁) (λ n, (sig₁.lean_type_of n)) → vector bool n₁ → Π n₂:ℕ, parlang.state n₂ (state sig₂) (λ n, (sig₂.lean_type_of n)) → vector bool n₂ → Prop) := 
+    (Q : Π n₁:ℕ, parlang.state n₁ (state sig₁) (parlang_mcl_global sig₁) → vector bool n₁ → Π n₂:ℕ, parlang.state n₂ (state sig₂) (parlang_mcl_global sig₂) → vector bool n₂ → Prop) := 
 rel_hoare_state P (mclk_to_kernel k₁) (mclk_to_kernel k₂) Q
 
 inductive mclp (sig : signature)
-| intro (f : memory (λ n, (sig.lean_type_of n)) → ℕ) (k : mclk sig) : mclp
+| intro (f : memory (parlang_mcl_global sig) → ℕ) (k : mclk sig) : mclp
 
-def mclp_to_program {sig : signature} : mclp sig → parlang.program (state sig) (λ n, sig.lean_type_of n)
+def mclp_to_program {sig : signature} : mclp sig → parlang.program (state sig) (parlang_mcl_global sig)
 | (mclp.intro f k) := parlang.program.intro f (mclk_to_kernel k)
 
 end mcl
@@ -321,8 +333,8 @@ namespace tactic.interactive
 
 open mcl tactic
 
-meta def unfold_to_parlang : tactic unit := do
-    rw ``mclp_to_program
+-- meta def unfold_to_parlang : tactic unit := do
+--     rw ``mclp_to_program
     -- rw mclk_to_kernel,
     -- rw prepend_load_expr,
     -- rw load_global_vars_for_expr,
@@ -335,7 +347,9 @@ end tactic.interactive
 
 namespace mcl
 
-def empty_state {sig : signature} : state sig := λ name idx, 0
+open mclk
+
+def empty_state {sig : signature} : state sig := λ name idx, default (type_map (type_of (sig name)))
 
 -- we need an assumption on the signature, i.e. tid must be int
 def mcl_init {sig : signature} : ℕ → state sig := λ n : ℕ, empty_state.update' (show type_of (sig "tid") = type.int, by sorry) (show (sig "tid").type.dim = ([1] : vector ℕ 1).length, by sorry) n
@@ -344,10 +358,9 @@ def mclp_rel {sig₁ sig₂ : signature} (P) (p₁ : mclp sig₁) (p₂ : mclp s
 
 --def eq_assert (sig₁ : signature) : state_assert sig₁ sig₁ := λ n₁ s₁ ac₁ n₂ s₂ ac₂, n₁ = n₂ ∧ s₁ = s₂ ∧ ac₁ = ac₂
 
-example (P) (n) (expr) : mclk_rel P (tlocal_assign n expr)
-
 -- we have to show some sort of non-interference
-example {sig : signature} {n} {k₁} {P Q : state_assert sig sig} (h : sig "i" = int) (hpi : ∀ n₁ s₁ ac₁ n₂ s₂ ac₂, P n₁ s₁ ac₁ n₂ s₂ ac₂ → n₁ = n) : mclk_rel P k₁ (for "i" h 0 (λ s, s.get' h < n) (tlocal_assign "i" (var "i" (by refl) + (const_int 1 h))) k₁) Q := begin
+example {sig : signature} {n} {k₁} {P Q : state_assert sig sig} (h : sig "i" = { scope := scope.global, type := ⟨_, [0], type.int⟩}) (hpi : ∀ n₁ s₁ ac₁ n₂ s₂ ac₂, P n₁ s₁ ac₁ n₂ s₂ ac₂ → n₁ = n ∧ n₂ = 1) : 
+mclk_rel P k₁ (for "i" h _ 0 (λ s, s.get' h < n) (tlocal_assign "i" (var "i" (by refl) + (const_int 1 h))) k₁) Q := begin
     sorry
 end
 
