src/arrcp_mcl.lean
@@ -22,26 +22,30 @@ lemma i_is_tlocal : is_tlocal (sig "i") := by apply eq.refl
 lemma a_is_global : is_global (sig "a") := by apply eq.refl
 lemma tid_is_tlocal : is_tlocal (sig "tid") := by apply eq.refl
 
-def arrcp₁ : mclp sig := mclp.intro (λ m, 10) (mclk.global_assign "b" (expression.const_int 7 (by refl)))
+def read_i := (expression.tlocal_var "i" (λ_, 0) (show type_of (sig "i") = type.int, by apply eq.refl) (by refl) i_is_tlocal)
+def read_tid := (expression.tlocal_var "tid" (λ_, 0) (show type_of (sig "tid") = type.int, by apply eq.refl) (show (sig "tid").type.dim = 1, by apply eq.refl) tid_is_tlocal)
 
-def read_i := (expression.tlocal_var "i" (λ_, 1) (show type_of (sig "i") = type.int, by apply eq.refl) (by refl) i_is_tlocal)
-def read_tid := (expression.tlocal_var "tid" (λ_, 1) (show type_of (sig "tid") = type.int, by apply eq.refl) (show (sig "tid").type.dim = 1, by apply eq.refl) tid_is_tlocal)
+def arrcp₁ : mclp sig := mclp.intro (λ m, 100) (
+    mclk.global_assign "b" [read_tid] (by refl) (expression.global_var "a" (λ_, read_tid) (show type_of (sig "a") = type.int, by refl) (by refl) a_is_global)
+)
 
-def arrcp₂ : mclp sig := mclp.intro (λ m, 10) (mclk.for "i" (by refl) read_tid (read_i < 100) (mclk.tlocal_assign "i" [1] (show ((sig "i").type).dim = vector.length [1], by refl) (read_i + read_tid)) (
+
+def arrcp₂ : mclp sig := mclp.intro (λ m, 10) (mclk.for "i" (by refl) (by refl) read_tid (read_i < 100) (mclk.tlocal_assign "i" [1] (show ((sig "i").type).dim = vector.length [1], by refl) (read_i + read_tid)) (
     mclk.global_assign "b" [read_i] (by refl) (expression.global_var "a" (λ_, read_i) (show type_of (sig "a") = type.int, by refl) (by refl) a_is_global)
 ))
 
+#eval mclp_to_program arrcp₁
 #eval mclp_to_program arrcp₂
-#reduce mclp_to_program arrcp₂
+--#reduce mclp_to_program arrcp₂
 
 example (c) : mclp_to_program arrcp₁ = c := begin
     rw arrcp₁,
     rw [mclp_to_program, mclk_to_kernel, prepend_load_expr, load_global_vars_for_expr],
-    unfold append,
-    rw list.append,
-    rw parlang.list_to_kernel_seq,
+    repeat {rw list.append},
     repeat {rw list.foldl},
+    repeat {rw list.foldr},
 end
+
 
 #eval mclp_to_program arrcp₁
 #check ```(mclp_to_program arrcp₁)
@@ -57,7 +61,7 @@ meta def num_args : expr → nat
 #check `(X)
 #eval parlang.expr.repr `(X)
 
-example : mclp_rel (λ m₁ m₂, sorry) arrcp₁ arrcp₂ (λ m₁ m₂, sorry) := begin
+example : mclp_rel eq arrcp₁ arrcp₂ eq := begin
     
 end
 
